formal/inference/Can_Take.thy
@@ -31,8 +31,20 @@ lemma max_reg_cons: "max_reg (a # G) = max (GExp.max_reg a) (max_reg G)"
   apply (simp add: max_reg_def)
   by (metis (no_types, lifting) List.finite_set Max.insert Max.set_eq_fold fold.simps(1) id_apply list.simps(15) max.assoc set_empty)
 
-lemma max_none: "max None x = x"
-  by (meson less_option.elims(2) linorder_not_le max.absorb2 option.distinct(1))
+lemma max_reg_append_singleton: "max_reg (as@[bs]) = max (max_reg as) (max_reg [bs])"
+  apply (simp add: max_reg_def)
+  by (metis max.commute max_None_r)
+
+lemma max_reg_append: "max_reg (as@bs) = max (max_reg as) (max_reg bs)"
+proof(induct bs rule: rev_induct)
+  case Nil
+  then show ?case
+    by (simp add: Can_Take.max_reg_def max_None_r)
+next
+  case (snoc x xs)
+  then show ?case
+    by (metis append_assoc max.assoc max_reg_append_singleton)
+qed
 
 lemma max_lt_val: "max (GExp.max_input a) (Can_Take.max_input G) = Some i \<Longrightarrow> (GExp.max_input a) \<le> Some i"
   by (metis max.cobounded1)
@@ -67,71 +79,71 @@ lemma gexp_max_input_nor_aux: "x \<in> set (s1) \<Longrightarrow>
 lemma gexp_max_input_nor: "GExp.max_input (Nor g1 g2) = max (GExp.max_input g1) (GExp.max_input g2)"
   apply (simp add: GExp.max_input_def Let_def)
   apply safe
-    apply (simp add: max_none)
-   apply (simp add: max.commute max_none)
+    apply (simp add: max_None_l)
+   apply (simp add: max.commute max_None_l)
   using enumerate_gexp_inputs_list gexp_max_input_nor_aux by fastforce
 
 lemma gexp_max_reg_nor: "GExp.max_reg (Nor g1 g2) = max (GExp.max_reg g1) (GExp.max_reg g2)"
   apply (simp add: GExp.max_reg_def Let_def)
   apply safe
-    apply (simp add: max_none)
-   apply (simp add: max.commute max_none)
+    apply (simp add: max_None_l)
+   apply (simp add: max.commute max_None_l)
   by (metis enumerate_gexp_regs_list gexp_max_input_nor_aux)
 
 lemma max_input_Eq: "GExp.max_input (Eq a1 a2) = max (AExp.max_input a1) (AExp.max_input a2)"
   apply (simp add: AExp.max_input_def GExp.max_input_def Let_def)
   apply safe
-    apply (simp add: max_none)
-   apply (simp add: max.commute max_none)
+    apply (simp add: max_None_l)
+   apply (simp add: max.commute max_None_l)
   using enumerate_aexp_inputs_list gexp_max_input_nor_aux by fastforce
 
 lemma max_reg_Eq: "GExp.max_reg (Eq a1 a2) = max (AExp.max_reg a1) (AExp.max_reg a2)"
   apply (simp add: AExp.max_reg_def GExp.max_reg_def Let_def)
   apply safe
-    apply (simp add: max_none)
-   apply (simp add: max.commute max_none)
+    apply (simp add: max_None_l)
+   apply (simp add: max.commute max_None_l)
   by (metis enumerate_aexp_regs_list gexp_max_input_nor_aux)
 
 lemma max_input_Gt: "GExp.max_input (Gt a1 a2) = max (AExp.max_input a1) (AExp.max_input a2)"
   apply (simp add: AExp.max_input_def GExp.max_input_def Let_def)
   apply safe
-    apply (simp add: max_none)
-   apply (simp add: max.commute max_none)
+    apply (simp add: max_None_l)
+   apply (simp add: max.commute max_None_l)
   by (metis Un_commute enumerate_aexp_inputs_list gexp_max_input_nor_aux)
 
 lemma max_reg_Gt: "GExp.max_reg (Gt a1 a2) = max (AExp.max_reg a1) (AExp.max_reg a2)"
   apply (simp add: AExp.max_reg_def GExp.max_reg_def Let_def)
   apply safe
-    apply (simp add: max_none)
-   apply (simp add: max.commute max_none)
+    apply (simp add: max_None_l)
+   apply (simp add: max.commute max_None_l)
   by (metis enumerate_aexp_regs_list gexp_max_input_nor_aux inf_sup_aci(5))
 
 lemma max_input_Plus: "AExp.max_input (Plus a1 a2) = max (AExp.max_input a1) (AExp.max_input a2)"
   apply (simp add: AExp.max_input_def Let_def)
   apply safe
-    apply (simp add: max_none)
-   apply (simp add: max.commute max_none)
+    apply (simp add: max_None_l)
+   apply (simp add: max.commute max_None_l)
   using enumerate_aexp_inputs_list gexp_max_input_nor_aux by fastforce
 
 lemma max_input_Minus: "AExp.max_input (Minus a1 a2) = max (AExp.max_input a1) (AExp.max_input a2)"
   apply (simp add: AExp.max_input_def Let_def)
   apply safe
-    apply (simp add: max_none)
-   apply (simp add: max.commute max_none)
+    apply (simp add: max_None_l)
+   apply (simp add: max.commute max_None_l)
   using enumerate_aexp_inputs_list gexp_max_input_nor_aux by fastforce
 
 lemma max_reg_Minus: "AExp.max_reg (Minus a1 a2) = max (AExp.max_reg a1) (AExp.max_reg a2)"
   apply (simp add: AExp.max_reg_def Let_def)
   apply safe
-    apply (simp add: max_none)
-   apply (simp add: max.commute max_none)
+    apply (simp add: max_None_l)
+   apply (simp add: max.commute max_None_l)
   by (metis enumerate_aexp_regs_list gexp_max_input_nor_aux)
 
 lemma max_reg_Plus: "AExp.max_reg (Plus a1 a2) = max (AExp.max_reg a1) (AExp.max_reg a2)"
   apply (simp add: AExp.max_reg_def Let_def)
   apply safe
-    apply (simp add: max_none)
-   apply (simp add: max.commute max_none)
+    apply (simp add: max_None_l)
+   apply (simp add: max.commute max_None_l)
   by (metis enumerate_aexp_regs_list gexp_max_input_nor_aux)
 
 lemma max_input_I: "AExp.max_input (V (vname.I i)) = Some i"
@@ -210,6 +222,10 @@ next
     by (metis apply_guards(9) aval_take gexp_max_input_null)
 qed
 
+lemma gval_take_flip: "GExp.max_input g < Some a \<Longrightarrow>
+    gval g (join_ir (take a i) r) = gval g (join_ir i r)"
+  by (metis gval_take)
+
 lemma apply_guards_take_or_pad: "Can_Take.max_input G < Some a \<Longrightarrow>
        apply_guards G (join_ir i r) \<Longrightarrow>
        apply_guards (ensure_not_null a) (join_ir i r) \<Longrightarrow>
@@ -242,7 +258,7 @@ lemma satisfiable_can_take:
   by (simp add: apply_guards_take_or_pad)
 
 lemma max_is_none: "(max x y = None) = (x = None \<and> y = None)"
-  by (metis max.commute max_def max_none)
+  by (metis max.commute max_def max_None_l)
 
 lemma aval_no_reg_swap_regs:
   "AExp.max_input x < Some a \<Longrightarrow>
@@ -339,6 +355,51 @@ lemma simple_mutex_direct_subsumption:
   apply (simp add: simple_mutex_def)
   by (metis can_take_satisfiable no_choice_no_subsumption)
 
+(*
+lemma apply_guards_no_reg_swap_regs:
+  "max_reg G = None \<Longrightarrow>
+   max_input G < Some a \<Longrightarrow>
+   apply_guards G (join_ir i ra) \<Longrightarrow>
+   apply_guards (ensure_not_null a) (join_ir i ra) \<Longrightarrow>
+   apply_guards G (join_ir (take_or_pad i a) r)"
+proof(induct G)
+  case Nil
+  then show ?case
+    by (simp add: max_input_def)
+next
+  case (Cons g gs)
+  then show ?case
+    by (metis apply_guards_cons gval_no_reg_swap_regs max.strict_boundedE max_input_cons
+              max_is_none max_reg_cons not_null_length take_or_pad_def)
+qed
+*)
+
+lemma max_reg_none_set: "(max_reg G = None) = (\<forall>g \<in> set G. GExp.max_reg g = None)"
+proof(induct G)
+  case Nil
+  then show ?case
+    by (simp add: max_reg_def)
+next
+  case (Cons a G)
+  then show ?case
+    by (simp add: max_reg_cons max_is_None)
+qed
+
+lemma no_reg_apply_guards_swap_regs: "max_reg G = None \<Longrightarrow> apply_guards G (join_ir i r) = apply_guards G (join_ir i r')"
+  apply (simp add: apply_guards_def max_reg_none_set)
+  by (metis no_reg_gval_swap_regs)
+
+lemma max_reg_ensure_not_null: "max_reg (ensure_not_null a) = None"
+proof(induct a)
+  case 0
+  then show ?case
+    by (simp add: ensure_not_null_def max_reg_def)
+next
+  case (Suc a)
+  then show ?case
+    by (simp add: ensure_not_null_cons max_reg_append max_reg_def max_reg_gNot max_reg_Null max_reg_V)
+qed
+
 fun not_null :: "gexp \<Rightarrow> bool" where
   "not_null (Null x) = False" |
   "not_null (Nor x y) = (not_null x \<and> not_null y)" |
@@ -431,5 +492,232 @@ lemma aval_Num_apply_guards_not_null:
   apply clarify
   using need_aval_I aval_input2state_within_bounds
   using leD by fastforce
+
+definition negate :: "gexp list \<Rightarrow> gexp" where
+  "negate g = gNot (fold gAnd g (Bc True))"
+
+lemma "\<not>\<^sub>? a \<or>\<^sub>? b = \<not>\<^sub>? (a \<or>\<^sub>? b)"
+  by simp
+
+lemma gval_fold_gAnd_append_singleton: "gval (fold gAnd (a @ [G]) (Bc True)) s = gval (fold gAnd a (Bc True)) s \<and>\<^sub>? gval G s "
+  apply (simp add: fold_conv_foldr del: foldr.simps)
+  by (simp only: foldr.simps comp_def gval_gAnd times_trilean_commutative)
+
+lemma gval_fold_rev_true: "gval (fold gAnd (rev G) (Bc True)) s = true \<Longrightarrow> gval (fold gAnd G (Bc True)) s = true"
+  by (simp add: fold_apply_guards apply_guards_def)
+
+lemma gval_fold_not_invalid_all_valid_contra:
+  "\<exists>g \<in> set G. gval g s = invalid \<Longrightarrow> gval (fold gAnd G (Bc True)) s = invalid"
+proof(induct G rule: rev_induct)
+  case Nil
+  then show ?case
+    by simp
+next
+  case (snoc a G)
+  then show ?case
+    apply (simp only: gval_fold_gAnd_append_singleton)
+    apply simp
+    using maybe_and_valid by blast
+qed
+
+lemma gval_fold_not_invalid_all_valid: "gval (fold gAnd G (Bc True)) s \<noteq> invalid \<Longrightarrow> \<forall>g \<in> set G. gval g s \<noteq> invalid"
+  using gval_fold_not_invalid_all_valid_contra by blast
+
+lemma all_gval_not_false: "(\<forall>g \<in> set G. gval g s \<noteq> false) = (\<forall>g \<in> set G. gval g s = true) \<or> (\<exists>g \<in> set G. gval g s = invalid)"
+  using trilean.exhaust by auto
+
+lemma must_have_one_false_contra: "\<forall>g \<in> set G. gval g s \<noteq> false \<Longrightarrow> gval (fold gAnd G (Bc True)) s \<noteq> false"
+  using all_gval_not_false[of G s]
+  apply simp
+  apply (case_tac "(\<forall>g\<in>set G. gval g s = true)")
+  using apply_guards_fold apply_guards_foldr gval_foldr_true apply auto[1]
+  by (simp add: gval_fold_not_invalid_all_valid_contra)
+
+lemma must_have_one_false: "gval (fold gAnd G (Bc True)) s = false \<Longrightarrow> \<exists>g \<in> set G. gval g s = false"
+  using must_have_one_false_contra by blast
+
+lemma all_valid_must_be_true_or_false: "(\<forall>g \<in> set G. gval g s \<noteq> invalid) = (\<forall>g \<in> set G. gval g s = true) \<or> (\<exists>g \<in> set G. gval g s = false)"
+  using all_gval_not_false by auto
+
+lemma all_valid_fold: "\<forall>g \<in> set G. gval g s \<noteq> invalid \<Longrightarrow> gval (fold gAnd G (Bc True)) s \<noteq> invalid"
+proof(induct G rule: rev_induct)
+  case Nil
+  then show ?case
+    by simp
+next
+  case (snoc a G)
+  then show ?case
+    apply (simp add: fold_conv_foldr del: foldr.simps)
+    apply (simp only: foldr.simps comp_def gval_gAnd)
+    by (simp add: maybe_and_invalid)
+qed
+
+lemma one_false_all_valid_false: "\<exists>g\<in>set G. gval g s = false \<Longrightarrow> \<forall>g\<in>set G. gval g s \<noteq> invalid \<Longrightarrow> gval (fold gAnd G (Bc True)) s = false"
+proof(induct G rule: rev_induct)
+  case Nil
+  then show ?case
+    by simp
+next
+  case (snoc x xs)
+  then show ?case
+    apply (simp add: fold_conv_foldr del: foldr.simps)
+    apply (simp only: foldr.simps comp_def gval_gAnd)
+    apply (case_tac "gval x s = false")
+     apply simp
+     apply (case_tac "gval (foldr gAnd (rev xs) (Bc True)) s")
+       apply simp
+      apply simp
+     apply simp
+    using all_valid_fold
+     apply (simp add: fold_conv_foldr)
+    apply simp
+    by (metis maybe_not.cases times_trilean.simps(5))
+qed
+
+lemma gval_fold_rev_false: "gval (fold gAnd (rev G) (Bc True)) s = false \<Longrightarrow> gval (fold gAnd G (Bc True)) s = false"
+  using must_have_one_false[of "rev G" s]
+        gval_fold_not_invalid_all_valid[of "rev G" s]
+  by (simp add: one_false_all_valid_false)
+
+lemma fold_invalid_means_one_invalid: "gval (fold gAnd G (Bc True)) s = invalid \<Longrightarrow> \<exists>g \<in> set G. gval g s = invalid"
+  using all_valid_fold by blast
+
+lemma gval_fold_rev_invalid: "gval (fold gAnd (rev G) (Bc True)) s = invalid \<Longrightarrow> gval (fold gAnd G (Bc True)) s = invalid"
+  using fold_invalid_means_one_invalid[of "rev G" s]
+  by (simp add: gval_fold_not_invalid_all_valid_contra)
+
+lemma gval_fold_rev_equiv_fold: "gval (fold gAnd (rev G) (Bc True)) s =  gval (fold gAnd G (Bc True)) s"
+  apply (cases "gval (fold gAnd (rev G) (Bc True)) s")
+    apply (simp add: gval_fold_rev_true)
+   apply (simp add: gval_fold_rev_false)
+  by (simp add: gval_fold_rev_invalid)
+
+lemma gval_fold_equiv_fold_rev: "gval (fold gAnd G (Bc True)) s = gval (fold gAnd (rev G) (Bc True)) s"
+  by (simp add: gval_fold_rev_equiv_fold)
+
+lemma gval_fold_gAnd: "gval (fold gAnd G (Bc True)) s = fold (\<and>\<^sub>?) (map (\<lambda>g. gval g s) G) true"
+proof(induct G rule: rev_induct)
+  case Nil
+  then show ?case
+    by simp
+next
+  case (snoc a G)
+  then show ?case
+    apply (simp add: fold_conv_foldr del: foldr.simps)
+    by (simp only: foldr.simps comp_def gval_gAnd)
+qed
+
+lemma gval_fold_equiv_gval_foldr: "gval (fold gAnd G (Bc True)) s = gval (foldr gAnd G (Bc True)) s"
+proof -
+  have "gval (fold gAnd G (Bc True)) s = gval (fold gAnd (rev G) (Bc True)) s"
+    using gval_fold_equiv_fold_rev by force
+then show ?thesis
+by (simp add: foldr_conv_fold)
+qed
+
+lemma gval_foldr_equiv_gval_fold: "gval (foldr gAnd G (Bc True)) s = gval (fold gAnd G (Bc True)) s"
+  by (simp add: gval_fold_equiv_gval_foldr)
+
+lemma gval_negate_cons: "gval (negate (a # G)) s = gval (gNot a) s \<or>\<^sub>? gval (negate G) s"
+  apply (simp only: negate_def gval_gNot gval_fold_equiv_gval_foldr)
+  by (simp only: foldr.simps comp_def gval_gAnd de_morgans_2)
+
+lemma maybe_or_true: "(x \<or>\<^sub>? y = true) = ((x = true \<or> y = true) \<and> x \<noteq> invalid \<and> y \<noteq> invalid)"
+  using plus_trilean.elims by blast
+
+lemma not_true: "(x \<noteq> true) = (x = false \<or> x = invalid)"
+  by (metis (no_types, lifting) maybe_not.cases trilean.distinct(1) trilean.distinct(3))
+
+lemma negate_true_guard: "(gval (negate G) s = true) = (gval (fold gAnd G (Bc True)) s = false)"
+  by (metis (no_types, lifting) gval_gNot maybe_double_negation maybe_not.simps(1) negate_def)
+
+lemma maybe_or_true_not_invalid: "(true \<or>\<^sub>? x = true) = (x \<noteq> invalid)"
+  by (simp add: maybe_or_true)
+
+lemma gval_negate_not_invalid: "(gval (negate gs) (join_ir i ra) \<noteq> invalid) = (gval (fold gAnd gs (Bc True)) (join_ir i ra) \<noteq> invalid)"
+  using gval_gNot maybe_not_invalid negate_def by auto
+
+lemma gval_fold_swap_regs: "max_reg G = None \<Longrightarrow> gval (fold gAnd G (Bc True)) (join_ir i r) = gval (fold gAnd G (Bc True)) (join_ir i r')"
+proof(induct G)
+  case Nil
+  then show ?case
+    by simp
+next
+  case (Cons a G)
+  then show ?case
+    apply (simp only: gval_fold_equiv_gval_foldr foldr.simps comp_def gval_gAnd)
+    by (metis (no_types, lifting) max_is_None max_reg_cons no_reg_gval_swap_regs)
+qed
+
+lemma negate_valid: "(\<not>\<^sub>? x \<noteq> invalid) = (x \<noteq> invalid)"
+  by (simp add: maybe_not_invalid)
+
+lemma maybe_and_false: "(x \<and>\<^sub>? y = false) = ((x = false \<or> y = false) \<and> x \<noteq> invalid \<and> y \<noteq> invalid)"
+  using times_trilean.elims by blast
+
+lemma gval_fold_cons: "gval (fold gAnd (g # gs) (Bc True)) s = gval g s \<and>\<^sub>? gval (fold gAnd gs (Bc True)) s"
+  apply (simp only: apply_guards_fold gval_fold_equiv_gval_foldr)
+  by (simp only: foldr.simps comp_def gval_gAnd)
+
+lemma maybe_and_not_invalid: "(x \<and>\<^sub>? y \<noteq> invalid) = (x \<noteq> invalid \<and> y \<noteq> invalid)"
+  by (simp add: maybe_and_invalid)
+
+lemma negate_not_apply_guards: "gval (negate G) s = true \<Longrightarrow> \<not> apply_guards G s"
+  by (simp add: apply_guards_fold negate_true_guard)
+
+lemma less_eq_length_trans: "max_input G < Some a \<Longrightarrow> a \<le> length i \<Longrightarrow> max_input G \<le> Some (length i)"
+  by (meson leD less_option.simps(4) not_le_imp_less order.strict_trans)
+
+lemma gval_fold_take:
+  "Can_Take.max_input G < Some a \<Longrightarrow>
+   a \<le> length i \<Longrightarrow>
+   Can_Take.max_input G \<le> Some (length i) \<Longrightarrow>
+   gval (fold gAnd G (Bc True)) (join_ir i r) = gval (fold gAnd G (Bc True)) (join_ir (take a i) r)"
+proof(induct G)
+  case Nil
+  then show ?case
+    by simp
+next
+  case (Cons g gs)
+  then show ?case
+    apply (simp only: gval_fold_cons)
+    apply (simp add: max_input_cons)
+    using gval_take[of g a i r]
+    by simp
+qed
+
+
+lemma gval_fold_take_false_not_true:
+  "Can_Take.max_reg G = None \<Longrightarrow>
+   Can_Take.max_input G < Some a \<Longrightarrow>
+   gval (fold gAnd G (Bc True)) (join_ir i ra) = false \<Longrightarrow>
+   a \<le> length i \<Longrightarrow>
+   gval (fold gAnd G (Bc True)) (join_ir (take a i) r) \<noteq> true"
+  using less_eq_length_trans[of G a i]
+  apply (simp add: gval_fold_swap_regs[of G i ra r])
+  by (simp add: gval_fold_take)
+
+lemma quick_negation_aux: "Can_Take.max_reg G = None \<Longrightarrow>
+    Can_Take.max_input G < Some a \<Longrightarrow>
+    \<exists>i r. gval (negate G) (join_ir i r) = true \<and> apply_guards (ensure_not_null a) (join_ir i r) \<Longrightarrow>
+    \<exists>i. length i = a \<and> \<not> apply_guards G (join_ir i r)"
+  apply clarify
+  apply (rule_tac x="take_or_pad i a" in exI)
+  apply (simp add: length_take_or_pad)
+  apply (simp add: apply_guards_ensure_not_null_length take_or_pad_def negate_true_guard)
+  apply (simp add: apply_guards_fold)
+  by (simp add: gval_fold_take_false_not_true)
+
+lemma quick_negation:
+  "max_reg (Guard t) = None \<Longrightarrow>
+   max_input (Guard t) < Some (Arity t) \<Longrightarrow>
+   satisfiable_list (negate (Guard t) # ensure_not_null (Arity t)) \<Longrightarrow>
+   \<exists>i. length i = Arity t \<and> \<not> apply_guards (Guard t) (join_ir i r)"
+  apply (simp add: satisfiable_list_def satisfiable_def fold_apply_guards apply_guards_cons del: fold.simps)
+  by (simp add: quick_negation_aux)
+
+definition "satisfiable_negation t = (max_reg (Guard t) = None \<and>
+   max_input (Guard t) < Some (Arity t) \<and>
+   satisfiable_list (negate (Guard t) # ensure_not_null (Arity t)))"
 
 end
